\documentclass{article}
\usepackage{blindtext}
\usepackage[paperheight=8.5in,paperwidth=22in,margin=1in,heightrounded]{geometry}

\usepackage{graphicx}
\usepackage{multicol}
   \usepackage{amsmath}
   \usepackage{hyperref}
   	

\oddsidemargin=-.3in
\evensidemargin=-.5in
\textwidth=20in
\topmargin=-.9in
\textheight=8.5in

\parindent=0in
\pagestyle{empty}


\usepackage{graphicx}
\usepackage{graphbox}
\usepackage{multicol}
\usepackage{amsmath}
\usepackage{mathtools}
\usepackage{pgfplots}
\usepackage{cancel}

\oddsidemargin=0in
\evensidemargin=-.5in
\textwidth= 15in
\topmargin=-1in
\textheight=7.5in

\parindent=.3in
\pagestyle{plain}


\everymath{\displaystyle}

\newenvironment{problems}
{
\begin{enumerate}
\renewcommand{\labelenumi}{ {\bf \arabic{enumi}}.}
\setlength{\itemsep}{1pt}
}
{
\end{enumerate}
}


\begin{document}


\begin{centering}
{\Huge \bf\boldmath $\displaystyle \frac{d}{dx}\left(x^n\right) \,=\,   nx^{n-1}$ \unboldmath} \smallskip

%{\Large \em Nueva Math 3}

\end{centering}

\vspace{3pc}

\noindent
$$\begin{array}{r c c c c c c c c c c}
\text{the derivative of $x^2$: }\quad & \frac{\left(x+h\right)^2 - x^2}{h} &=& \frac{\left( x^2 + {\color{blue}2xh} {\color{red} + h^2}\right) - x^2}{h} &=& \frac{ {\color{blue}2xh} {\color{red} + h^2} }{h} &=&  {\color{blue}2x} {\color{red} + h} & \xrightarrow[\text{reeeally small}]{\text{as h gets}} & {\color{blue}2x} \\ \\
\text{the derivative of $x^3$: }\quad &  \frac{\left(  x+h\right)^3 - x^3}{h} &=& \frac{\left(  x^3 + {\color{blue}3x^2h} {\color{red}+ 3xh^2 + h^3}\right) - x^3}{h} &=& \frac{ {\color{blue}3x^2h} {\color{red}+ 3xh^2 + h^3} }{h}  &=&   {\color{blue}3x^2} {\color{red}+ 3xh + h^2} & \xrightarrow[\text{reeeally small}]{\text{as h gets}} & {\color{blue}3x^2} \\ \\
\text{the derivative of $x^4$: }\quad &\frac{\left(x+h\right)^4 - x^4}{h} &=& \frac{\left( x^4 + {\color{blue}4x^3h }{\color{red}+ 6x^2h^2 + 4xh^3 + h^4}\right) - x^4}{h} &=& \frac{ {\color{blue}4x^3h }{\color{red}+ 6x^2h^2 + 4xh^3 + h^4} }{h}  &=&  {\color{blue}4x^3 }{\color{red}+ 6x^2h + 4xh^2 + h^3} & \xrightarrow[\text{reeeally small}]{\text{as h gets}} & {\color{blue}4x^3} \\ \\
\text{the derivative of $x^5$: }\quad &\frac{\left( x+h\right)^5 - x^5}{h} &=&\displaystyle\frac{\left( x^5 + {\color{blue}5x^4h }{\color{red}+ 10x^3h^2 + 10x^2h^3 + 5xh^4 + h^5}\right) - x^5}{h} &=&\displaystyle\frac{ {\color{blue}5x^4h }{\color{red}+ 10x^3h^2 + 10x^2h^3 + 5xh^4  +h^5 } }{h} &=&  {\color{blue}5x^4 }{\color{red}+ 10x^3h + 10x^2h^2 + 5xh^3  + h^4}  & \xrightarrow[\text{reeeally small}]{\text{as h gets}} & {\color{blue}5x^4} \\ \\  \\ \\
\vdots &\vdots && \vdots && \vdots && \vdots & &\vdots \\ \\ \\ \\
\text{the derivative of $x^n$: }\quad & \frac{(x+h)^n-x^n}{h} &=& \frac{\left(x^n \,+\, {\color{blue}nx^{n-1}h} \,+\, {\color{red}  \left({\color{red}\substack{\text{a bunch of cross terms}\\\text{with $x$'s and $h$'s}} }\right)} \,\right) -x^n}{h}  &=& \frac{ {\color{blue}nx^{n-1}h} +    {\color{red}  \left({\color{red}\substack{\text{a bunch of cross terms}\\\text{with $x$'s and $h$'s}} }\right)} \,    }{h} &=& {\color{blue}nx^{n-1}} + {\color{red} \left(\substack{\text{a bunch of cross terms}\\\text{with $x$'s and $h$'s, but}\\\text{with the $h$ power}\\\text{down by $1$}} \right)  } & \xrightarrow[\text{reeeally small}]{\text{as h gets}} & {\color{blue}nx^{n-1}} \\ \\ \\ \\
 & &=& \frac{\left(x^n \,+\, {\color{blue}nx^{n-1}h} \,+\, {\color{red} {n\choose n-2} x^{n-2}h^2 + {n\choose n-3} x^{n-3}h^3 + \cdots + {n\choose 2} + nxh^{n-1} + h^n }\right)  \, -x^n}{h}  &=& \frac{ {\color{blue}nx^{n-1}h} +    {\color{red} {n\choose n-2} x^{n-2}h^2 + {n\choose n-3} x^{n-3}h^3 + \cdots + {n\choose 2} + nxh^{n-1} + h^n } \,    }{h} &=& {\color{blue}nx^{n-1}} + {\color{red} {n\choose n-2} x^{n-2}h + {n\choose n-3} x^{n-3}h^2 + \cdots + {n\choose 2} + nxh^{n-2} + h^{n-1}  } & \xrightarrow[\text{reeeally small}]{\text{as h gets}} & {\color{blue}nx^{n-1}} \\ \\ \\ \\
 &= \frac{  \overbrace{\left(\sum\limits_{k=0}^{k=n}{n\choose {n-k}}x^{n-k}h^{k} \right) }^{\text{the binomial theorem!!!}}  - x^n}{h} &=& \displaystyle \frac{ \left( x^{n} + {\color{blue} {n\choose {n-1}}x^{n-1}h^{1}} \,\,+ {\color{red} \sum\limits_{k=2}^{k=n}{n\choose {n-k}}x^{n-k}h^{k} } \right) \quad-\quad x^n}{h}   &=& \displaystyle\frac{ {\color{blue} nx^{n-1}h} \,\,+{\color{red} \sum\limits_{k=2}^{k=n}{n\choose {n-k}}x^{n-k}h^{k} } } {h}  &=& {\color{blue} nx^{n-1} } \,\,+{\color{red} \sum\limits_{k=2}^{k=n}{n\choose {n-k}}x^{n-k}h^{k-1} }    & \xrightarrow[\text{reeeally small}]{\text{as h gets}} & {\color{blue}nx^{n-1}}
\end{array}$$


\end{document}