---
title: Sequence problems!!!!
usemathjax: true
layout: post
---


For each of the following sequences, write out the first few terms, and then determine whether it converges or diverges. If it converges, what does it converge to? 

<div style="column-width: 10em;  column-gap: 2em;">
<ol class='problems'>
<li> $\displaystyle S_n = \frac{1-n}{n^2}$ </li>
<li> $\displaystyle f(n) = \frac{1}{n!}$ </li>
<li> $\displaystyle f(n) = \frac{1}{n} + 7$ </li>
<li> $\displaystyle f(n) = \frac{1}{2^n}$ </li>
<li> $\displaystyle f(n) = \frac{1}{\ln(n)}$ </li>
<li> $\displaystyle f(n) = \frac{n!}{2^n}$ </li>
<li> $\displaystyle f(n) = \frac{2^n}{n!}$ </li>
<li> $\displaystyle f(n) = \frac{n^2}{n!}$ </li>
<li> $\displaystyle f(n) = \frac{n^2}{n!} + 2$ </li>
<li> $\displaystyle f(n) = \frac{n!}{n^2}$ </li>
<li> $\displaystyle f(n) = \frac{\ln(n)}{n^2}$ </li>
<li> $\displaystyle f(n) = \frac{n^2}{\ln(n)}$ </li>
<li> $\displaystyle f(n) = \frac{\sqrt{n}}{\ln(n)}$ </li>
<li> $\displaystyle f(n) = \frac{\ln(n)}{\sqrt{n}}$ </li>
<li> $\displaystyle f(n) = \frac{(-1)^{n+1}}{2n-1}$ </li>
<li> $S_n = 2 + (-1)^n$ </li>
<li> $S_n = 2 + (0.1)^n$ </li>
<li> $S_n = 2 + (-0.1)^n$ </li>
<li> $S_n = 2 + (1)^n$ </li>
<li> $S_n = (-1)^n$ </li>
<li> $\displaystyle f(n) = \frac{1}{(-1)^n}$ </li>
<li> $\displaystyle S_n = \frac{n + (-1)^n}{n}$ </li>
<li> $\displaystyle S_n = 4 - \frac{3}{n^2}$ </li>
<li> $\displaystyle S_n = \frac{1-2n}{1+2n}$ </li>
<li> $\displaystyle f(n) = \frac{2n+1}{1-3\sqrt{n}}$ </li>
<li> $\displaystyle S_n = \frac{1-5n^4}{n^4 + 8n^3}$ </li>
<li> $\displaystyle f(n) = \frac{n+3}{n^2 + 5n + 6}$ </li>
<li> $\displaystyle f(n) = \frac{n^2 - 2n + 1}{n-1}$ </li>
<li> $\displaystyle f(n) = \frac{5n^3+1}{10n^3-3n^2+7}$ </li>
<li> $\displaystyle S_n = \frac{1-n^3}{70-4n^2}$ </li>
<li> $S_n = 1 + (-1)^n$ </li>
<li> $\displaystyle f(n) = (-1)^n \left( 1-\frac{1}{n} \right)$ </li>
<li> $\displaystyle S_n = \left( \frac{n+1}{2n} \right) \left( 1- \frac{1}{n} \right)$ </li>
<li> $\displaystyle S_n = \left( 2 - \frac{1}{2^n} \right) \left( 3+\frac{1}{2^n} \right)$ </li>
<li> $\displaystyle f(n) = \frac{(-1)^{n+1}}{2n-1}$ </li>
<li> $\displaystyle S_n = \left(-\frac{1}{2} \right)^n$ </li>
<li> $\displaystyle f(n) = \frac{\sin(n)}{n}$ </li>
<li> $\displaystyle f(n) = \frac{\sin^2(n)}{2^n}$ </li>
<li> $\displaystyle S_n = \sqrt{\frac{2n}{n+1}}$ </li>
<li> $\displaystyle f(n) = \sin\left(\frac{\pi}{2} + \frac{1}{n}\right)$ </li>
<li> $f(n) = \ln(n) - \ln(n+1)$ </li>
<li> $\displaystyle f(n) = \frac{n}{2^n}$ </li>
<li> $\displaystyle f(n) = \frac{3^n}{n^3}$ </li>
<li> $\displaystyle f(n) = \frac{\ln(n+1)}{\sqrt{n}}$ </li>
<li> $\displaystyle f(n) = \frac{\ln(n)}{\ln(2n)}$ </li>
<li> $f(n) = 8^{1/n}$ </li>
<li> $f(n) = (0.03)^{1/n}$ </li>
<li> $\displaystyle f(n) =\frac{(n+1)!}{n}$ </li>
<li> $\displaystyle f(n) =\frac{(3n-1)!}{(3n+1)!}$ </li>
</ol>
</div>